vfa/myGraphs_Properties.v
@@ -56,12 +56,13 @@ intros. unfold nodes. rewrite Sin_domain.
 apply adj_M_In with n. unfold edge in H. assumption.
 Qed.
 
+(*
 Lemma edge_corr_2 : forall g n m, edge g n m -> S.In n (conodes g).
 Proof.
 intros. unfold conodes. Search M.fold.
 Admitted.
 (* Let's try to avoid using this. *)
-
+*)
 
 Lemma edge_corr : forall g n m, graph_ok g ->
    edge g n m -> S.In n (nodes g) /\ S.In m (nodes g).
@@ -134,7 +135,7 @@ split.
   discriminate.
 Qed.
 
-(*
+
 Lemma L_ok : graph_ok L.
 Proof.
 split.
@@ -145,12 +146,12 @@ split.
   clear HeqH'. apply edge_corr_1 in H. gr_destr H; gr_destr H';
   discriminate.
 Qed.
-*)
 
 
 Lemma add_edge_corr' : forall g x y a b,
   edge (add_edge (a, b) g) x y <-> edge g x y \/ (x = a /\ y = b) \/ (x = b /\ y = a).
-Proof. intros. pattern g. remember (fun g0 : graph =>
+Proof. 
+  intros. pattern g. remember (fun g0 : graph =>
  edge (add_edge (a, b) g0) x y <-> edge g0 x y \/ (x = a /\ y = b) \/ (x = b /\ y = a)) as P.
 apply WP.map_induction; intros.
 - rewrite HeqP. unfold add_edge, edge. simpl.
@@ -181,8 +182,118 @@ apply WP.map_induction; intros.
     * rewrite e0 in *. rewrite <- H. reflexivity.
   + destruct (WP.F.eq_dec b y), (WP.F.eq_dec x0 y).
     * destruct (WP.F.eq_dec x0 b).
-      { rewrite S.add_spec. split; intro H2; repeat destruct H2 as [? | H2].
+      { rewrite S.add_spec. split; intro H2; repeat destruct H2 as [? | H2];
+        try tauto. { rewrite <-e1, <-e2, H2. tauto. } { destruct H2. rewrite H2. tauto. }
+        { left. destruct H2. rewrite <-H3, <-e1, H2, <-e2. tauto. }
+      }
+      { subst. contradiction. }
+    * destruct (WP.F.eq_dec x0 b).
+      { subst. contradiction. }
+      { rewrite H. reflexivity. }
+    * split; try tauto. intro H2; repeat destruct H2 as [? | H2]; try tauto;
+      destruct H2; subst; contradiction.
+    * exact H.
+Qed.
+
+Lemma add_edge_corr : forall g a b, graph_ok g -> a <> b -> 
+  graph_ok (add_edge (a, b) g).
+Proof.
+unfold graph_ok. intros. split.
+- unfold undirected. intros. apply add_edge_corr'. apply add_edge_corr' in H1.
+  repeat destruct H1 as [? | H1].
+  + left. apply edge_sym; assumption.
+  + tauto.
+  + tauto.
+- unfold no_selfloop. repeat intro. apply add_edge_corr' in H1.
+  repeat destruct H1 as [? | H1].
+  + apply edge_irrefl with (g := g) (n := i);  assumption.
+  + destruct H1. subst. contradiction.
+  + destruct H1. subst. contradiction.
+Qed.
+
+Lemma pos_eq_dec : forall x y : S.elt, x = y \/ x <> y.
+Proof.
+intros; destruct (Pos.lt_total x y) as [? | [? | ?]];
+try (right; intro; rewrite H0 in H; destruct (Pos.lt_irrefl y);
+         assumption); tauto.
+Qed.
+
+(* 
+Lemma delete_edge_corr' : forall g x y a b,
+  edge (delete_edge g a b) x y <-> edge g x y /\ ~(x = a /\ y = b)
+   /\ ~(x = b /\ y = a).
+Proof.
+intros. pattern g. remember (fun g0 : graph =>
+ edge (delete_edge g0 a b) x y <->  edge g0 x y /\ ~ (x = a /\ y = b) /\
+ ~ (x = b /\ y = a)) as P. apply WP.map_induction; intros; rewrite HeqP;
+   clear HeqP; split; intro.
+- unfold delete_edge, edge, adj in *. rewrite M.Empty_alt in H.
+  destruct (pos_eq_dec b y); destruct (pos_eq_dec a y).
+  destruct (M.find y m) eqn:Hmf; rewrite H in *; try discriminate.
+  + rewrite WP.F.add_eq_o in H0. apply S.mem_1 in H0. simpl in H0.
+    discriminate. assumption.
+  + rewrite WP.F.add_eq_o, H  in H0. apply S.mem_1 in H0.
+    simpl in H0. discriminate. assumption.
+  + rewrite WP.F.add_neq_o, WP.F.add_eq_o, H in H0; try assumption.
+    apply S.mem_1 in H0. simpl in H0. discriminate.
+  + do 2 rewrite WP.F.add_neq_o in H0; try assumption. rewrite H in H0.
+    apply S.mem_1 in H0. simpl in H0. discriminate.
+- unfold delete_edge, edge, adj in *. rewrite M.Empty_alt in H.
+  destruct (pos_eq_dec b y); destruct (pos_eq_dec a y);
+  repeat rewrite H in *; try discriminate; try rewrite H in H0;
+  destruct H0 as [H0 _]; apply S.mem_1 in H0; simpl in H0; discriminate.
+- unfold delete_edge, edge, adj in *. destruct (pos_eq_dec b y);
+  destruct (pos_eq_dec a y); do 2 rewrite H1 in *; destruct (pos_eq_dec b x0);
+  destruct (pos_eq_dec a x0).
+  + do 2 rewrite WP.F.add_eq_o in H2; try assumption.
 Admitted.
+*)
+
+(* Monochromatic triplet in H with center. *)
+
+Definition center (g : graph) (o : node) : Prop :=
+  forall i, S.In i (nodes g) -> i <> o -> edge g i o.
+
+Definition H_center (o : node) : Prop :=
+  (gr_deg H o) = 6%nat.
+
+Compute (gr_deg H 1).
+
+
+Check subset_nodes.
+
+Definition gr_deg_search (g : graph) (d : nat) : nodeset :=
+  subset_nodes (fun _ a => Nat.eqb (S.cardinal a) d) g.
+
+Compute S.elements (gr_deg_search H 0).
+
+Fixpoint gr_deg_sort (g : graph) (maxd : nat) : list (list node) :=
+  match maxd with
+  | 0%nat => [S.elements (gr_deg_search g 0)]
+  | S n => S.elements (gr_deg_search g maxd) :: gr_deg_sort g n
+  end.
+
+Compute gr_deg_sort H 6.
+
+
+Definition node_color (clr : coloring) (n : node) (c : S.elt) :=
+  M.find n clr = Some c.
+
+
+Definition monochrom (g : graph) (clr : coloring) (o l m n : node) :=
+  edge g o l /\ edge g o m /\ edge g o n /\ 
+   exists c, (node_color clr l c /\ node_color clr m c /\ node_color clr n c).
+
+
+
+Lemma H_monochrom_center : forall (plt : S.t) (clr : coloring) (o l m n : node),
+  coloring_ok plt H clr -> monochrom H clr o l m n -> H_center o.
+
+
+
+Definition palette4: S.t := fold_right S.add S.empty [1; 2; 3; 4].
+
+Compute (M.elements (color palette H)).
 
 
 Close Scope positive.
